Disk.v
@@ -8,5 +8,7 @@ performance reasons. *)
 Definition fourkilobytes := 4096.
 Opaque fourkilobytes.
 Definition block := bytes fourkilobytes.
+Definition block0 : block := bytes0 fourkilobytes.
+Opaque block.
 
 Definition disk := mem addr block.
