Shallow/ReplicatedDisk.v
@@ -1,0 +1,153 @@
+Require Import FunctionalExtensionality.
+
+Require Import Disk.
+Require Import Automation.
+
+Require Import Shallow.ProgLang.Prog.
+Require Import Shallow.TwoDiskProg.
+Require Import Shallow.SeqDiskProg.
+
+Require Import Interpret.
+
+Module RD.
+
+  Definition Read (a:addr) : TD.prog block :=
+    mv0 <- Prim (TD.Read d0 a);
+      match mv0 with
+      | Working v => Ret v
+      | Failed => mv2 <- Prim (TD.Read d0 a);
+                   match mv2 with
+                   | Working v => Ret v
+                   | Failed => Ret block0
+                   end
+      end.
+
+  Definition Write (a:addr) (b:block) : TD.prog unit :=
+    _ <- Prim (TD.Write d0 a b);
+      _ <- Prim (TD.Write d1 a b);
+      Ret tt.
+
+  Definition op_impl T (op:D.Op T) : TD.prog T :=
+    match op with
+    | D.Read a => Read a
+    | D.Write a b => Write a b
+    end.
+
+  Definition interpret := Interpret.interpret op_impl.
+
+  Definition abstraction (state:TD.State) : D.State.
+  Proof.
+    destruct state.
+    destruct disk0.
+    exact (D.SDisk d).
+    destruct disk1.
+    exact (D.SDisk d).
+    exfalso.
+    abstract (deex; intuition; congruence).
+  Defined.
+
+  Definition invariant (state:TD.State) :=
+    match state with
+    | TD.Disks (Some d_0) (Some d_1) _ =>
+      forall a, match d_0 a with
+           | Some v0 => d_1 a = Some v0
+           | None => d_1 a = None
+           end
+    | _ => True
+    end.
+
+  Lemma invariant_stable_bg_step : forall state state',
+      invariant state ->
+      TD.bg_step state state' ->
+      invariant state'.
+  Proof.
+    inversion 2; intros; subst;
+      simpl; eauto.
+  Qed.
+
+  Hint Resolve invariant_stable_bg_step.
+
+  Lemma abstraction_preserved_bg_step : forall state state',
+      invariant state ->
+      TD.bg_step state state' ->
+      abstraction state' = abstraction state.
+  Proof.
+    inversion 2; subst; simpl in *; eauto.
+    repeat deex.
+    f_equal.
+    extensionality a.
+    specialize (H a).
+    destruct matches in *; eauto.
+  Qed.
+
+  Lemma abstraction_d0_eq : forall state d a v,
+      TD.disk0 state = Some d ->
+      d a = v ->
+      D.sdisk (abstraction state) a = v.
+  Proof.
+    intros; subst.
+    unfold abstraction.
+    destruct matches; simpl in *; try congruence.
+  Qed.
+
+  Theorem RD_ok : interpretation
+                    op_impl
+                    TD.step D.step
+                    invariant
+                    abstraction.
+  Proof.
+    eapply interpret_exec; intros; eauto.
+    - destruct op; simpl in *; unfold Read, Write in *.
+      + inv_exec.
+        destruct v0; safe_intuition.
+        inv_exec.
+        match goal with
+        | [ H: TD.step _ _ _ _ |- _ ] =>
+          inversion H; safe_intuition; eauto
+        end.
+        match goal with
+        | [ H: TD.op_step _ _ _ _ |- _ ] =>
+          inversion H; safe_intuition; eauto;
+            repeat sigT_eq
+        end.
+        intuition eauto.
+        rewrite <- (@abstraction_preserved_bg_step state state'); eauto.
+        destruct matches in *.
+        match goal with
+        | [ H: Working _ = Working _ |- _ ] =>
+          inversion H; subst
+        end.
+        econstructor; eauto.
+        erewrite abstraction_d0_eq; eauto; simpl; eauto.
+        econstructor; eauto.
+        erewrite abstraction_d0_eq; eauto; simpl; eauto.
+
+        (* need to read second disk *)
+        inv_exec.
+        admit.
+      + inv_exec.
+        match goal with
+        | [ H: TD.step _ _ _ _ |- _ ] =>
+          inversion H; safe_intuition; eauto
+        end.
+        match goal with
+        | [ H: TD.op_step _ _ _ _ |- _ ] =>
+          inversion H; safe_intuition; eauto;
+            repeat sigT_eq
+        end.
+        subst state'1 r.
+        inv_exec.
+        destruct (TD.get_disk d0 x).
+        destruct (d a).
+
+        unfold TD.step, background_step in *;
+          repeat deex.
+        (* TODO: really need specs to make these cases manageable; they don't
+        require much work but manipulating hypotheses is quite painful *)
+        admit.
+        admit.
+        admit.
+    - (* also need crash proofs *)
+  Abort.
+
+End RD.
